ExistentialRules/Terms.lean
@@ -1,0 +1,13 @@
+/-
+Copyright 2026 Lukas Gerlach
+Released under Apache 2.0 license as described in the file LICENSE.
+-/
+
+module
+
+import ExistentialRules.Terms.Basic
+import ExistentialRules.Terms.Cyclic
+import ExistentialRules.Terms.GroundTerm
+import ExistentialRules.Terms.ListsOfTerms
+import ExistentialRules.Terms.SkolemTerm
+
