ExistentialRules/Terms/GroundTerm.lean
@@ -1,0 +1,274 @@
+/-
+Copyright 2026 Lukas Gerlach
+Released under Apache 2.0 license as described in the file LICENSE.
+-/
+
+module
+
+public import BasicLeanDatastructures.FiniteTree
+import BasicLeanDatastructures.List.Basic
+
+public import ExistentialRules.Terms.SkolemTerm
+
+/-!
+# Ground Terms
+
+A `GroundTerm` is a constant or a functional term with arbitrary nesting of function symbols (`SkolemFS`).
+Aiming to define `GroundTerm`, we need to define a more basic structure first, where we do not demand yet that function symbol arities are respected.
+`PreGroundTerm`s need to be able to model Skolem terms, i.e. function terms. We can represent those conveniently using inductively defined `FiniteTree`s.
+
+With `PreGroundTerm`s in place, we merely define `GroundTerm`s to be the `PreGroundTerm`s where `arity_ok` holds.
+We then define appropriate constructors and recursion principles on the `GroundTerm` to make it behave almost like an inductive type with a `GroundTerm.const` and `GroundTerm.func` constructor.
+-/
+
+public section
+
+/-- The `PreGroundTerm` is simply a `FiniteTree (SkolemFS sig) sig.C`. That is a tree that features Skolem function symbols in its inner nodes and constants in its leaf nodes. -/
+abbrev PreGroundTerm (sig : Signature) [DecidableEq sig.C] [DecidableEq sig.V] := FiniteTree (SkolemFS sig) sig.C
+
+namespace PreGroundTerm
+
+/-- The arity of a functional term is ok if the defined arity of its function symbol matches its number of children and `arity_ok` also holds for each child. For constants, i.e. the leaf nodes, the arity is trivially ok. -/
+@[expose]
+def arity_ok {sig : Signature} [DecidableEq sig.C] [DecidableEq sig.V] : FiniteTree (SkolemFS sig) sig.C -> Bool
+| .leaf _ => true
+| .inner func ts =>
+  ts.length == func.arity && ts.attach.all (fun ⟨t, _⟩ => arity_ok t)
+
+end PreGroundTerm
+
+/-- As mentioned above, a `GroundTerm` is simply a `PreGroundTerm` subtype where `arity_ok` holds. -/
+abbrev GroundTerm (sig : Signature) [DecidableEq sig.C] [DecidableEq sig.V] := { t : PreGroundTerm sig // PreGroundTerm.arity_ok t }
+
+
+namespace GroundTerm
+
+variable {sig : Signature} [DecidableEq sig.C] [DecidableEq sig.V]
+
+/-- A `GroundTerm` can be direclty constructed from a constant. -/
+@[expose]
+def const (c : sig.C) : GroundTerm sig := ⟨FiniteTree.leaf c, by simp [PreGroundTerm.arity_ok]⟩
+
+/-- The `GroundTerm.const` constructor is injective. -/
+@[grind inj]
+theorem const.inj : Function.Injective (GroundTerm.const (sig := sig)) := by intro c d; unfold const; simp
+@[simp]
+theorem const.injEq {c d : sig.C} : GroundTerm.const c = GroundTerm.const d ↔ c = d := by grind
+
+/-- Also, a `GroundTerm` can be constructed from a `SkolemFS` and a list of `GroundTerm`s as long as the length of the list matches the function symbol's arity. -/
+@[expose]
+def func (func : SkolemFS sig) (ts : List (GroundTerm sig)) (arity_ok : ts.length = func.arity) : GroundTerm sig := ⟨FiniteTree.inner func ts.unattach, by
+  unfold PreGroundTerm.arity_ok
+  rw [Bool.and_eq_true, beq_iff_eq]
+  constructor
+  . rw [List.length_unattach]; exact arity_ok
+  . rw [List.all_eq_true]
+    intro t t_mem
+    unfold List.unattach at t_mem
+    rw [List.attach_map, List.mem_map] at t_mem
+    rcases t_mem with ⟨t, t_mem, t_eq⟩
+    rw [← t_eq]
+    exact t.val.property
+⟩
+
+/-- The `GroundTerm.func` constructor is injective. -/
+@[grind ->]
+theorem func.inj
+  {func1 func2 : SkolemFS sig} {ts1 ts2 : List (GroundTerm sig)} {arity_ok1 : ts1.length = func1.arity} {arity_ok2 : ts2.length = func2.arity} :
+  GroundTerm.func func1 ts1 arity_ok1 = GroundTerm.func func2 ts2 arity_ok2 -> func1 = func2 ∧ ts1 = ts2 := by unfold func; simp
+@[simp]
+theorem func.injEq
+  {func1 func2 : SkolemFS sig} {ts1 ts2 : List (GroundTerm sig)} {arity_ok1 : ts1.length = func1.arity} {arity_ok2 : ts2.length = func2.arity} :
+  GroundTerm.func func1 ts1 arity_ok1 = GroundTerm.func func2 ts2 arity_ok2 ↔ func1 = func2 ∧ ts1 = ts2 := by grind
+
+/-- `GroundTerm.func` can never be equal to `GroundTerm.const`. -/
+theorem func_neq_const {func : SkolemFS sig} {ts : List (GroundTerm sig)} {arity_ok : ts.length = func.arity} {c : sig.C} :
+  GroundTerm.func func ts arity_ok ≠ GroundTerm.const c := by simp [GroundTerm.func, const]
+
+/-- A term cannot occur in its own child. -/
+theorem eq_while_contained_is_impossible {func : SkolemFS sig} {ts : List (GroundTerm sig)} {arity_ok : ts.length = func.arity} :
+    GroundTerm.func func ts arity_ok ∉ ts := by
+  intro mem
+  apply FiniteTree.tree_eq_while_contained_is_impossible (GroundTerm.func func ts arity_ok).val ts.unattach func
+  . rfl
+  . rw [List.mem_unattach]; exact ⟨_, mem⟩
+
+/-- We define a cases eliminator for the `GroundTerm` having a case for each constructor. This allows to use the `cases` tactic direcly on `GroundTerm`s. -/
+@[elab_as_elim, cases_eliminator]
+def cases
+    {motive : GroundTerm sig -> Sort u}
+    (t : GroundTerm sig)
+    (const : (c : sig.C) -> motive (GroundTerm.const c))
+    (func : (func : SkolemFS sig) -> (ts : List (GroundTerm sig)) -> (arity_ok : ts.length = func.arity) -> motive (GroundTerm.func func ts arity_ok)) :
+    motive t :=
+  match eq : t.val with
+  | .leaf c =>
+    have eq : t = GroundTerm.const c := Subtype.ext eq
+    eq ▸ const c
+  | .inner f ts =>
+    let ts : List (GroundTerm sig) := ts.attach.map (fun t' => ⟨t'.val, by
+      have prop := t.property
+      unfold PreGroundTerm.arity_ok at prop
+      simp only [eq, Bool.and_eq_true, beq_iff_eq] at prop
+      have prop := prop.right
+      rw [List.all_eq_true] at prop
+      apply prop ⟨t', t'.property⟩
+      apply List.mem_attach
+    ⟩)
+    have arity_ok : ts.length = f.arity := by
+      have prop := t.property
+      unfold PreGroundTerm.arity_ok at prop
+      simp only [eq, Bool.and_eq_true, beq_iff_eq] at prop
+      unfold ts
+      rw [List.length_map, List.length_attach]
+      exact prop.left
+    have eq : t = GroundTerm.func f ts arity_ok := by
+      apply Subtype.ext
+      unfold GroundTerm.func
+      simp only [eq, ts]
+      unfold List.unattach
+      rw [List.map_map, List.map_attach_eq_pmap]
+      simp
+    eq ▸ (func f ts arity_ok)
+
+/-- We define an induction eliminator for the `GroundTerm` having a case for each constructor. This allows to use the `induction` tactic direcly on `GroundTerm`s. -/
+@[elab_as_elim, induction_eliminator]
+def rec
+    {motive : GroundTerm sig -> Sort u}
+    (const : (c : sig.C) -> motive (GroundTerm.const c))
+    (func : (func : SkolemFS sig) -> (ts : List (GroundTerm sig)) -> (arity_ok : ts.length = func.arity) -> (∀ t, t ∈ ts -> motive t) -> motive (GroundTerm.func func ts arity_ok))
+    (t : GroundTerm sig) :
+    motive t :=
+  match eq_val : t.val with
+  | .leaf c =>
+    have eq : t = GroundTerm.const c := Subtype.ext eq_val
+    eq ▸ const c
+  | .inner f ts =>
+    let ts : List (GroundTerm sig) := ts.attach.map (fun t' => ⟨t'.val, by
+      have prop := t.property
+      unfold PreGroundTerm.arity_ok at prop
+      simp only [eq_val, Bool.and_eq_true, beq_iff_eq] at prop
+      have prop := prop.right
+      rw [List.all_eq_true] at prop
+      apply prop ⟨t', t'.property⟩
+      apply List.mem_attach
+    ⟩)
+    have arity_ok : ts.length = f.arity := by
+      have prop := t.property
+      unfold PreGroundTerm.arity_ok at prop
+      simp only [eq_val, Bool.and_eq_true, beq_iff_eq] at prop
+      unfold ts
+      rw [List.length_map, List.length_attach]
+      exact prop.left
+    have eq : t = GroundTerm.func f ts arity_ok := by
+      apply Subtype.ext
+      unfold GroundTerm.func
+      simp only [eq_val, ts]
+      unfold List.unattach
+      rw [List.map_map, List.map_attach_eq_pmap]
+      simp
+    eq ▸ (func f ts arity_ok (by
+      intro t' mem
+      have : t'.val.depth < t.val.depth := by
+        conv => right; unfold FiniteTree.depth
+        simp only [eq_val]
+        rw [Nat.add_comm]
+        apply Nat.lt_add_one_of_le
+        apply List.le_max?_getD_of_mem
+        apply List.mem_map_of_mem
+        rw [List.mem_map] at mem
+        rcases mem with ⟨s, s_mem, t_eq⟩
+        rw [← t_eq]
+        unfold List.attach at s_mem
+        unfold List.attachWith at s_mem
+        rw [List.mem_pmap] at s_mem
+        rcases s_mem with ⟨_, s_mem, s_eq⟩
+        rw [← s_eq]
+        exact s_mem
+      apply GroundTerm.rec const func
+    ))
+termination_by t.val.depth
+
+/-- A `GroundTerm` that has been constructed from a constant can be converted into this constants again. -/
+def toConst (t : GroundTerm sig) (isConst : ∃ c, t = GroundTerm.const c) : sig.C :=
+  match eq : t.val with
+  | .leaf c => c
+  | .inner _ _ => by
+    apply False.elim
+    rcases isConst with ⟨c, isConst⟩
+    rw [isConst] at eq
+    simp [GroundTerm.const] at eq
+
+/-- For a `GroundTerm` that has been constructed as a functional term, we can obtain the function symbol. -/
+def functionSymbol (t : GroundTerm sig) (isFunc : ∃ func ts arity_ok, t = GroundTerm.func func ts arity_ok) : SkolemFS sig :=
+  match eq : t.val with
+  | .leaf _ => by apply False.elim; rcases isFunc with ⟨func, ts, arity_ok, eq2⟩; rw [eq2] at eq; simp [GroundTerm.func] at eq
+  | .inner func _ => func
+
+/-- The `depth` of a `GroundTerm` is the depth of the underlying `FiniteTree`, i.e. the deepest nesting of function symbols (+1). -/
+@[expose]
+def depth (t : GroundTerm sig) : Nat := t.val.depth
+
+/-- The `constants` occurring in a `GroundTerm` are exactly the leaves of the underlying `FiniteTree`. -/
+@[expose]
+def constants (t : GroundTerm sig) : (List sig.C) := t.val.leaves
+
+/-- The `functions` (i.e. function symbols `SkolemFS`) occurring in a `GroundTerm` are exactly the inner labels of the underlying `FiniteTree`. -/
+@[expose]
+def functions (t : GroundTerm sig) : (List (SkolemFS sig)) := t.val.innerLabels
+
+/-- Applying `toConst` to a `GroundTerm.const` yields exactly the contained constant. -/
+@[simp, grind =]
+theorem toConst_const {c : sig.C} : (GroundTerm.const c).toConst (by exists c) = c := by rfl
+
+/-- Applying `functionSymbol` to a `GroundTerm.func` yields exactly the contained function symbol. -/
+@[simp, grind =]
+theorem functionSymbol_func {func : SkolemFS sig} {ts : List (GroundTerm sig)} {arity_ok : ts.length = func.arity} :
+  (GroundTerm.func func ts arity_ok).functionSymbol (by exists func, ts, arity_ok) = func := by rfl
+
+/-- Constants have `depth` 1. -/
+@[simp, grind =]
+theorem depth_const {c : sig.C} : (GroundTerm.const c).depth = 1 := by
+  simp [GroundTerm.const, depth, FiniteTree.depth]
+
+/-- The `depth` of a function term is the maximum depth of its children + 1. -/
+@[simp, grind =]
+theorem depth_func {f : SkolemFS sig} {ts : List (GroundTerm sig)} {arity_ok : ts.length = f.arity} :
+    (GroundTerm.func f ts arity_ok).depth = 1 + (((ts.map (GroundTerm.depth)).max?).getD 1) := by
+  simp only [GroundTerm.func, depth, FiniteTree.depth]
+  have : ts.map depth = ts.unattach.map FiniteTree.depth := by rw [List.map_unattach]; rfl
+  rw [this]
+
+/-- Every term has a depth greater zero since constants already have depth 1. -/
+theorem depth_gt_zero {t : GroundTerm sig} : 0 < t.depth := by cases t <;> grind
+
+/-- The `constants` of a constant are the singleton list with the constant itself. -/
+@[simp, grind =]
+theorem constants_const {c : sig.C} : (GroundTerm.const c).constants = [c] := by
+  simp [GroundTerm.const, constants, FiniteTree.leaves]
+
+/-- The `constants` of a function term are the constants of its children. -/
+@[simp, grind =]
+theorem constants_func {f : SkolemFS sig} {ts : List (GroundTerm sig)} {arity_ok : ts.length = f.arity} :
+    (GroundTerm.func f ts arity_ok).constants = ts.flatMap GroundTerm.constants := by
+  simp only [GroundTerm.func, constants, FiniteTree.leaves]
+  rw [List.flatMap_unattach]
+  rfl
+
+/-- A constant has no `functions`. -/
+@[simp, grind =]
+theorem functions_const {c : sig.C} : (GroundTerm.const c).functions = [] := by
+  simp [GroundTerm.const, functions, FiniteTree.innerLabels]
+
+/-- The `functions` of a function term consist of the function symbol of the current term and the function symbols of all its children. -/
+@[simp, grind =]
+theorem functions_func {f : SkolemFS sig} {ts : List (GroundTerm sig)} {arity_ok : ts.length = f.arity} :
+    (GroundTerm.func f ts arity_ok).functions = f :: (ts.flatMap GroundTerm.functions) := by
+  simp only [GroundTerm.func, functions, FiniteTree.innerLabels]
+  rw [List.cons_eq_cons]
+  constructor
+  . rfl
+  . rw [List.flatMap_unattach]; rfl
+
+end GroundTerm
+
